lib/pulse/lib/Pulse.Lib.BigAnchoredReference.fsti
@@ -86,6 +86,16 @@ val gather2' (#a:Type) (#p:_) (#anc:_) (r:ref a p anc) (#v1 #v2:erased a)
         (pts_to_full r #(half_perm full_perm) v1 ** pts_to_full r #(half_perm full_perm) v2)
         (fun _ -> pts_to_full r v1 ** pure (v1 == v2))
 
+val share4' (#a:Type) (#p:_) (#anc:_) (r:ref a p anc) (#v:erased a)
+  : stt_ghost unit
+        (pts_to_full r #(half_perm full_perm) v)
+        (fun _ -> pts_to_full r #(half_perm (half_perm full_perm)) v ** pts_to_full r #(half_perm (half_perm full_perm)) v)
+
+val gather4' (#a:Type) (#p:_) (#anc:_) (r:ref a p anc) (#v1 #v2:erased a)
+  : stt_ghost unit
+        (pts_to_full r #(half_perm (half_perm full_perm)) v1 ** pts_to_full r #(half_perm (half_perm full_perm)) v2)
+        (fun _ -> pts_to_full r #(half_perm full_perm) v1 ** pure (v1 == v2))
+
 val write (#a:Type) (#p:_) (#anc:_) (r:ref a p anc) (#v:erased a) (w : erased a)
   : stt_ghost unit
         (pts_to r v ** pure (p v w /\ (forall anchor. anc anchor v ==> anc anchor w)))
