share/pulse/examples/NuPool.fsti
@@ -12,11 +12,27 @@ type vcode : Type u#3 = {
 
 val handle : Type u#0
 
-
 val pool (code:vcode) : Type u#0
 val pool_alive (#[T.exact (`full_perm)] f : perm) (#code:vcode) (p:pool code) : vprop
 
+val big_joinable (#code:vcode) (p:pool code) (post:erased code.t) (h : handle) : vprop
 val joinable (#code:vcode) (p:pool code) (post:erased code.t) (h : handle) : vprop
+
+val pool_done (#code:vcode) (p:pool code) : vprop
+
+val joinable_is_small (#code:vcode) (p:pool code) (post:erased code.t) (h : handle) 
+  : Lemma (is_small (joinable p post h))
+          [SMTPat (joinable p post h)]
+
+val big_spawn
+  (#code:vcode)
+  (p : pool code)
+  (#pf : perm)
+  (#pre : erased code.t)
+  (#post : erased code.t)
+  (f : unit -> stt unit (code.up pre) (fun _ -> code.up post))
+  : stt handle (pool_alive #pf p ** code.up pre)
+               (fun h -> pool_alive #pf p ** big_joinable p post h)
 
 val spawn
   (#code:vcode)
@@ -28,7 +44,13 @@ val spawn
   : stt handle (pool_alive #pf p ** code.up pre)
                (fun h -> pool_alive #pf p ** joinable p post h)
 
-val pool_done (#code:vcode) (p:pool code) : vprop
+val big_disown
+  (#code:vcode)
+  (#p : pool code)
+  (#post : erased code.t)
+  (h : handle)
+  : stt_ghost unit (big_joinable p post h)
+                   (fun _ -> pledge [] (pool_done p) (code.up post))
 
 val disown
   (#code:vcode)
@@ -36,10 +58,10 @@ val disown
   (#post : erased code.t)
   (h : handle)
   : stt_ghost unit (joinable p post h)
-                   (fun _ -> pledge [] (pool_done p) (code.up post))
+                   (fun _ -> pledge [] (pool_done p) (code.up post)) // TODO: SmallPledge
 
 (* spawn + disown *)
-val spawn_
+val big_spawn_
   (#code:vcode)
   (p : pool code)
   (#pf : perm)
@@ -48,6 +70,43 @@ val spawn_
   (f : unit -> stt unit (code.up pre) (fun _ -> code.up post))
   : stt unit (pool_alive #pf p ** code.up pre)
              (fun _ -> pool_alive #pf p ** pledge [] (pool_done p) (code.up post))
+
+val spawn_
+  (#code:vcode)
+  (p : pool code)
+  (#pf : perm)
+  (#pre : erased code.t)
+  (#post : erased code.t)
+  (f : unit -> stt unit (code.up pre) (fun _ -> code.up post))
+  : stt unit (pool_alive #pf p ** code.up pre)
+             (fun _ -> pool_alive #pf p ** pledge [] (pool_done p) (code.up post)) // TODO: SmallPledge
+
+val big_try_await
+  (#code:vcode)
+  (#p : pool code)
+  (#post : erased code.t)
+  (h : handle)
+  (#f : perm)
+  : stt bool (pool_alive #f p ** big_joinable p post h)
+             (fun ok -> pool_alive #f p ** (if ok then code.up post else big_joinable p post h))
+
+val big_await
+  (#code:vcode)
+  (#p : pool code)
+  (#post : erased code.t)
+  (h : handle)
+  (#f : perm)
+  : stt unit (pool_alive #f p ** big_joinable p post h)
+             (fun _ -> pool_alive #f p ** code.up post)
+
+val try_await
+  (#code:vcode)
+  (#p : pool code)
+  (#post : erased code.t)
+  (h : handle)
+  (#f : perm)
+  : stt bool (pool_alive #f p ** joinable p post h)
+             (fun ok -> pool_alive #f p ** (if ok then code.up post else joinable p post h))
 
 val await
   (#code:vcode)
